Restructure invocation properties and fix proofs
Pull out the definitions of requirements for the different cases of
capability invocations into separate definitions, rather than having one
huge property, which was getting unwieldy.

Fix the monotonicity proof and the tooling for verifying concrete ISAs.

model/isabelle/Capabilities_lemmas.thy
@@ -70,6 +70,15 @@ locale Capabilities =
     and is_tagged_cap_of_mem_bytes[simp]: "\<And>c bytes tag. cap_of_mem_bytes_method CC bytes tag = Some c \<Longrightarrow> is_tagged_method CC c \<longleftrightarrow> tag = B1"
 begin
 
+abbreviation "is_tagged c \<equiv> is_tagged_method CC c"
+abbreviation "is_sealed c \<equiv> is_sealed_method CC c"
+abbreviation "get_cursor c \<equiv> get_cursor_method CC c"
+abbreviation "seal c t \<equiv> seal_method CC c t"
+abbreviation "unseal c \<equiv> unseal_method CC c"
+abbreviation "clear_global c \<equiv> clear_global_method CC c"
+abbreviation "is_sentry c \<equiv> is_sentry_method CC c"
+abbreviation "get_indirect_sentry_type c \<equiv> get_indirect_sentry_type_method CC c"
+
 inductive_set derivable :: "'cap set \<Rightarrow> 'cap set" for C :: "'cap set" where
   Copy: "c \<in> C \<Longrightarrow> c \<in> derivable C"
 | Restrict: "c' \<in> derivable C \<Longrightarrow> leq_cap CC c c' \<Longrightarrow> c \<in> derivable C"
